MyOCL.thy
@@ -31,7 +31,7 @@ fun transAs :: "MyOCL.as \<Rightarrow> MySQL.col" where
 fun evalWithCtx :: "OCLexp \<Rightarrow> Objectmodel \<Rightarrow> OCLexp \<Rightarrow> val \<Rightarrow> val" where
 "evalWithCtx (MyOCL.Int i) om var val = VInt i"
 (* For the time being *)
-| "evalWithCtx (MyOCL.Var x) om (MyOCL.IVar i) val = (VString x)"
+| "evalWithCtx (MyOCL.Var x) om (MyOCL.IVar i) val = (VObj x)" 
 | "evalWithCtx (MyOCL.IVar x) om (MyOCL.IVar i) val = val"
 (* *)
 | "evalWithCtx (MyOCL.Eq e1 e2) om var val = 
@@ -41,7 +41,7 @@ VBool (equalVal (evalWithCtx e1 om var val) (evalWithCtx e2 om var val))"
 else (VList (projValList (Col (transAtt att)) [extPerson v (getPersonList om)])))"
 | "evalWithCtx (MyOCL.As (Var v) as) om (MyOCL.IVar i) val
 = (if (v=i) then (projVal (Col (transAs as)) val) 
-else (VList (extCol v (transAs as) (getEnrollmentList om))))"
+else (VList (extCol (MySQL.Var v) (transAs as) (getEnrollmentList om))))"
 | "evalWithCtx (MyOCL.Size exp) om var val
 = VList [VInt (sizeVal (evalWithCtx exp om var val))]"
 | "evalWithCtx (MyOCL.IsEmpty exp) om var val
@@ -57,10 +57,10 @@ fun filterWithBody :: "val list \<Rightarrow> OCLexp \<Rightarrow> OCLexp \<Righ
 
 fun eval :: "OCLexp \<Rightarrow> Objectmodel \<Rightarrow> val list" where
 "eval (MyOCL.Int i) om = [VInt i]"
-| "eval (MyOCL.Var x) om = [VString x]"
+| "eval (MyOCL.Var x) om = [VObj x]"
 | "eval (MyOCL.Eq e1 e2) om = [VBool (equalValList (eval e1 om) (eval e2 om))]" 
 (*| "eval (MyOCL.Att (Var v) att) om = projValList (Col (transAtt att)) [extPerson v (getPersonList om)]"*)
-(*| "eval (MyOCL.As (Var v) as) om = extCol v (transAs as) (getEnrollmentList om)"*)
+| "eval (MyOCL.As (Var v) as) om = extCol (MySQL.Var v) (transAs as) (getEnrollmentList om)"
 | "eval (MyOCL.Size exp) om = [VInt (sizeValList (eval exp om))]"
 | "eval (MyOCL.IsEmpty exp) om = [VBool (isEmptyValList (eval exp om))]"
 | "eval (MyOCL.Exists src v body) om = [VBool (\<not> isEmptyValList (filterWithBody (eval src om) v body om))]"
